SortExperiments/QSortHoareMo3.lean
@@ -7,15 +7,15 @@ import Quicksort.Init.Ord
 
 variable
   [Ord α]
-  -- [ile_trans : Std.TransOrd α]
+  [ile_trans : Std.TransOrd α]
 
 
 open Ord
 
 @[inline]
 public def qsort_hoare_mo3 (arr : Array α) /- (left : Nat := 0) -/ /- (right := arr.size - 1) -/
-    (not_lt : ∀ {x y : α}, ¬(compare y x |>.isLT) ↔ (compare x y |>.isLE) := by grind)
-    (le_trans : ∀ {x y z : α}, (compare x y).isLE → (compare y z).isLE → (compare x z).isLE := by grind)
+    -- (not_lt : ∀ {x y : α}, ¬lt y x ↔ le x y := by grind)
+    -- (le_trans : ∀ {x y z : α}, le x y → le y z → le x z := by grind)
     : Array α :=
   let rec @[specialize]
   recurse {n} (as : Vector α n) (left : Nat) (right: Nat) (hsize' : right ≤ n - 1) : Vector α n :=
@@ -23,8 +23,8 @@ public def qsort_hoare_mo3 (arr : Array α) /- (left : Nat := 0) -/ /- (right :=
       have hr : right < n := by omega
 
       let v := Pivot.median_of_three as left right hlr hr
-      have : ¬(compare v.piv' v.arr'[left] |>.isLT) ∧ ¬(compare v.arr'[right] v.piv' |>.isLT) :=
-        Pivot.median_of_three_sorted not_lt le_trans hlr hr
+      have : (¬lt v.piv' v.arr'[left]) ∧ (¬lt v.arr'[right] v.piv') :=
+        Pivot.median_of_three_sorted /- not_lt le_trans -/ hlr hr
 
       let ⟨⟨a, j', i'⟩, (_ : _ < i'), (_ : j' < _ )⟩ :=
         Partitioning.hoare v.arr' v.piv' left right hlr hr  this.left this.right
